wiring up framing in the prover

pulse/lib/steel/pulse/Pulse.Checker.Auto.Prover.fst
@@ -104,46 +104,34 @@ let init_prover_state (#g:env) (#ctxt:vprop) (ctxt_typing: vprop_typing g ctxt)
         proof_steps_typing=post_with_emp (proof_steps_idem_typing _ ctxt);
     }
 
-noeq
-type match_result g p ctxt = {
-  matched:list vprop;
-  unmatched:list vprop;
-  ctxt':list vprop;
-  p_eq: vprop_equiv g (list_as_vprop p) (list_as_vprop (unmatched @ matched));
-  ctxt_eq: vprop_equiv g (list_as_vprop ctxt) (list_as_vprop (ctxt' @ matched))
-}
-
 open FStar.List.Tot 
-
-assume
-val all_simple_matches (g:env) (p:list vprop) (ctxt:list vprop)
-  : T.Tac (option (match_result g p ctxt))
 
 let step_t = #g:_ -> #o:_ -> p:prover_state g o -> T.Tac (option (prover_state g o))
 
 let step_match : step_t = 
   fun #g #o (p:prover_state g o) ->
-    match all_simple_matches g p.unmatched_pre p.remaining_ctxt with
-    | None -> None
-    | Some res ->
+    let res = F.all_matches g p.unmatched_pre p.remaining_ctxt in
+    match res.matched with
+    | [] -> None
+    | _ ->
       let matched_pre = Tm_Star (list_as_vprop res.matched) p.matched_pre in
         // remaining_ctxt ~ res.ctxt' * res.matched
       let veq 
         : vprop_equiv_x g tm_unit 
                           (Tm_Star (list_as_vprop p.remaining_ctxt) p.matched_pre)
-                          (Tm_Star (list_as_vprop res.ctxt') matched_pre)
+                          (Tm_Star (list_as_vprop res.unmatched_q) matched_pre)
         = magic ()
       in
         // p.unmatched_pre ~ res.unmatched @ res.matched
       let pre_equiv
-          : vprop_equiv g (comp_pre p.c) (Tm_Star (list_as_vprop res.unmatched) matched_pre)
+          : vprop_equiv g (comp_pre p.c) (Tm_Star (list_as_vprop res.unmatched_p) matched_pre)
           = magic ()
       in
       let proof_steps_typing = st_typing_equiv_post p.proof_steps_typing veq in
       Some 
-        { p with unmatched_pre = res.unmatched;
+        { p with unmatched_pre = res.unmatched_p;
                  matched_pre;
-                 remaining_ctxt = res.ctxt';
+                 remaining_ctxt = res.unmatched_q;
                  proof_steps_typing;
                  pre_equiv }
 
